feat(Typ.Syn.): induction/recursion principle for action
This commit provides a new induction principle for TypedSyntax.action
which is more powerful than the default generated one.

Specifically, it provides additional induction hypotheses for the
'InternalCall' case. One for the functions body, and one for each
argument in the argument context.

coq/TypedSyntax.v
@@ -54,6 +54,220 @@ Section Syntax.
   | APos {sig tau} (pos: pos_t) (a: action sig tau)
     : action sig tau.
 
+  Definition acontext (sig argspec: tsig var_t) :=
+    context (fun k_tau => action sig (snd k_tau)) argspec.
+
+  (* This induction principle contains all necessary
+    hypothesis to do an actual induction over an `action`
+    without resorting to manual Fixpoint proofs.
+
+    Note that this principle can only be used on goals
+    of the form `Pa /\ Pargs` where `Pa` stand for an arbitrary
+    proposition over actions while `Pargs` represents an
+    analogus porp extended to contexts of actions (just
+      like they are used by `InternalCall`)
+
+    As an example, have a look at the proofs in Hoare.v
+  *)
+  Lemma action_ind_complete :
+    (* Propositions *)
+    forall P : forall {sig tau}, action sig tau -> Prop,
+    forall P' : forall {sig argspec}, acontext sig argspec -> Prop,
+
+    (* All cases for the normal action *)
+    (forall (sig : tsig var_t) (tau : type),
+      @P sig tau (Fail tau)) ->
+    (forall (sig : list (var_t * type)) (k : var_t) (tau : type) (m : member (k, tau) sig),
+      @P sig tau (Var m)) ->
+    (forall (sig : tsig var_t) (tau : type) (cst : tau),
+      @P sig tau (Const cst)) ->
+    (forall (sig : list (var_t * type)) (k : var_t) (tau : type) (m : member (k, tau) sig) (ex : action sig tau),
+      @P sig tau ex ->
+      @P sig unit_t (Assign m ex)) ->
+    (forall (sig : tsig var_t) (tau : type) (r1 : action sig unit_t) (r2 : action sig tau),
+      @P sig unit_t r1 ->
+      @P sig tau r2 ->
+      @P sig tau (Seq r1 r2)) ->
+    (forall (sig : tsig var_t) (tau tau' : type) (var : var_t) (ex : action sig tau) (body : action ((var, tau) :: sig) tau'),
+      @P sig tau ex ->
+      @P ((var, tau) :: sig) tau' body ->
+      @P sig tau' (Bind var ex body)) ->
+    (forall (sig : tsig var_t) (tau : type) (cond : action sig (bits_t 1)) (tbranch : action sig tau) (fbranch : action sig tau),
+      @P sig (bits_t 1) cond ->
+      @P sig tau tbranch ->
+      @P sig tau fbranch ->
+      @P sig tau (If cond tbranch fbranch)) ->
+    (forall (sig : tsig var_t) (port : Port) (idx : reg_t),
+      @P sig (R idx) (Read port idx)) ->
+    (forall (sig : tsig var_t) (port : Port) (idx : reg_t) (value : action sig (R idx)),
+      @P sig (R idx) value ->
+      @P sig unit_t (Write port idx value)) ->
+    (forall (sig : tsig var_t) (fn : fn1) (arg1 : action sig (arg1Sig (Sigma1 fn))),
+      @P sig (arg1Sig (Sigma1 fn)) arg1 ->
+      @P sig (retSig (Sigma1 fn)) (Unop fn arg1)) ->
+    (forall (sig : tsig var_t) (fn : fn2) (arg1 : action sig (arg1Sig (Sigma2 fn))) (arg2 : action sig (arg2Sig (Sigma2 fn))),
+      @P sig (arg1Sig (Sigma2 fn)) arg1 ->
+      @P sig (arg2Sig (Sigma2 fn)) arg2 ->
+      @P sig (retSig (Sigma2 fn)) (Binop fn arg1 arg2)) ->
+    (forall (sig : tsig var_t) (fn : ext_fn_t) (arg : action sig (arg1Sig (Sigma fn))),
+      @P sig (arg1Sig (Sigma fn)) arg ->
+      @P sig (retSig (Sigma fn)) (ExternalCall fn arg)) ->
+    (forall (sig : tsig var_t) (tau : type) (argspec : tsig var_t) (fn : InternalFunction' fn_name_t (action argspec tau)) (args : context (fun k_tau : var_t * type => action sig (snd k_tau)) argspec),
+      @P argspec tau fn.(int_body) ->
+      @P' sig argspec args ->
+      @P sig tau (InternalCall fn args)) ->
+    (forall (sig : tsig var_t) (tau : type) (pos : pos_t) (a : action sig tau),
+      @P sig tau a ->
+      @P sig tau (APos pos a)) ->
+
+    (* All cases for action contexts *)
+    (forall sig,
+      @P' sig [] CtxEmpty) ->
+    (forall sig n tau argspec a args,
+      @P sig tau a ->
+      @P' sig argspec args ->
+      @P' sig ((n,tau) :: argspec) (CtxCons (n,tau) a args)) ->
+
+    (* goal *)
+    (forall {sig tau} (a : action sig tau),
+    @P sig tau a) /\
+    (forall {sig argspec} (args : acontext sig argspec),
+    @P' sig argspec args).
+  Proof.
+    intros P P' H1 H2 H3 H4 H5 H6 H7 H8 H9 H10 H11 H12 H13 H14 H1' H2'.
+    assert (Hargs : (forall (sig : tsig var_t) (tau : type) (a : action sig tau), P sig tau a) -> forall (sig argspec : tsig var_t) (args : acontext sig argspec), P' sig argspec args).
+    + intro Ha. fix IH 3.
+      destruct args.
+      * apply H1'.
+      * destruct k.
+        apply H2'.
+        - apply Ha.
+        - apply IH.
+    + assert (Ha : forall (sig : tsig var_t) (tau : type) (a : action sig tau), P sig tau a).
+      * fix IH 3.
+        destruct a.
+        - apply H1.
+        - apply H2.
+        - apply H3.
+        - apply H4; apply IH.
+        - apply H5; apply IH.
+        - apply H6; apply IH.
+        - apply H7; apply IH.
+        - apply H8.
+        - apply H9. apply IH.
+        - apply H10. apply IH.
+        - apply H11; apply IH.
+        - apply H12. apply IH.
+        - apply H13. apply IH.
+          apply (Hargs IH).
+        - apply H14. apply IH.
+      * split.
+        - apply (Ha).
+        - apply (Hargs Ha).
+  Qed.
+
+  Definition action_rect_complete
+    (* Propositions *)
+    (P : forall {sig tau}, action sig tau -> Type)
+    (P' : forall {sig argspec}, acontext sig argspec -> Type)
+
+    (* All cases for the normal action *)
+    (f_fail : forall sig tau,
+      @P sig tau (Fail tau))
+    (f_var : forall sig k tau (m : member (k, tau) sig),
+      @P sig tau (Var m))
+    (f_const : forall sig tau cst,
+      @P sig tau (Const cst))
+    (f_assign : forall sig k tau (m : member (k, tau) sig) (ex : action sig tau),
+      @P sig tau ex ->
+      @P sig unit_t (Assign m ex))
+    (f_seq : forall sig tau (r1 : action sig unit_t) (r2 : action sig tau),
+      @P sig unit_t r1 ->
+      @P sig tau r2 ->
+      @P sig tau (Seq r1 r2))
+    (f_bind : forall sig (tau tau' : type) (var : var_t) (ex : action sig tau) (body : action ((var, tau) :: sig) tau'),
+      @P sig tau ex ->
+      @P ((var, tau) :: sig) tau' body ->
+      @P sig tau' (Bind var ex body))
+    (f_if : forall sig tau (cond : action sig (bits_t 1)) (tbranch : action sig tau) (fbranch : action sig tau),
+      @P sig (bits_t 1) cond ->
+      @P sig tau tbranch ->
+      @P sig tau fbranch ->
+      @P sig tau (If cond tbranch fbranch))
+    (f_read : forall sig (port : Port) (idx : reg_t),
+      @P sig (R idx) (Read port idx))
+    (f_write : forall sig (port : Port) (idx : reg_t) (value : action sig (R idx)),
+      @P sig (R idx) value ->
+      @P sig unit_t (Write port idx value))
+    (f_unop : forall sig (fn : fn1) (arg1 : action sig (arg1Sig (Sigma1 fn))),
+      @P sig (arg1Sig (Sigma1 fn)) arg1 ->
+      @P sig (retSig (Sigma1 fn)) (Unop fn arg1))
+    (f_binop : forall sig (fn : fn2) (arg1 : action sig (arg1Sig (Sigma2 fn))) (arg2 : action sig (arg2Sig (Sigma2 fn))),
+      @P sig (arg1Sig (Sigma2 fn)) arg1 ->
+      @P sig (arg2Sig (Sigma2 fn)) arg2 ->
+      @P sig (retSig (Sigma2 fn)) (Binop fn arg1 arg2))
+    (f_ext_call : forall sig (fn : ext_fn_t) (arg : action sig (arg1Sig (Sigma fn))),
+      @P sig (arg1Sig (Sigma fn)) arg ->
+      @P sig (retSig (Sigma fn)) (ExternalCall fn arg))
+    (f_int_call : forall sig (tau : type) (argspec : tsig var_t) (fn : InternalFunction' fn_name_t (action argspec tau)) (args : context (fun k_tau : var_t * type => action sig (snd k_tau)) argspec),
+      @P argspec tau fn.(int_body) ->
+      @P' sig argspec args ->
+      @P sig tau (InternalCall fn args))
+    (f_apos : forall sig (tau : type) (pos : pos_t) (a : action sig tau),
+      @P sig tau a ->
+      @P sig tau (APos pos a))
+
+    (* All cases for action contexts *)
+    (f_args_emtyp : forall sig,
+      @P' sig [] CtxEmpty)
+    (f_args_cons : forall sig n tau argspec a args,
+      @P sig tau a ->
+      @P' sig argspec args ->
+      @P' sig ((n,tau) :: argspec) (CtxCons (n,tau) a args))
+
+    : (* goal *)
+    (forall {sig tau} (a : action sig tau),
+    @P sig tau a) *
+    (forall {sig argspec} (args : acontext sig argspec),
+    @P' sig argspec args).
+  Proof.
+    (* intros P P' H1 H2 H3 H4 H5 H6 H7 H8 H9 H10 H11 H12 H13 H14 H1' H2'. *)
+    assert (Hargs : (forall (sig : tsig var_t) (tau : type) (a : action sig tau), P sig tau a) -> forall (sig argspec : tsig var_t) (args : acontext sig argspec), P' sig argspec args).
+    + intro Ha. fix IH 3.
+      destruct args.
+      * apply f_args_emtyp.
+      * destruct k.
+        apply f_args_cons.
+        - apply Ha.
+        - apply IH.
+    + assert (Ha : forall (sig : tsig var_t) (tau : type) (a : action sig tau), P sig tau a).
+      * fix IH 3.
+        destruct a.
+        - apply f_fail.
+        - apply f_var.
+        - apply f_const.
+        - apply f_assign; apply IH.
+        - apply f_seq; apply IH.
+        - apply f_bind; apply IH.
+        - apply f_if; apply IH.
+        - apply f_read.
+        - apply f_write. apply IH.
+        - apply f_unop. apply IH.
+        - apply f_binop; apply IH.
+        - apply f_ext_call. apply IH.
+        - apply f_int_call. apply IH.
+          apply (Hargs IH).
+        - apply f_apos. apply IH.
+      * split.
+        - apply (Ha).
+        - apply (Hargs Ha).
+  Defined.
+
+  Definition action_rec_complete
+    (P : forall sig tau, action sig tau -> Set)
+    (P' : forall sig argspec, acontext sig argspec -> Set) :=
+    action_rect_complete P P'.
+
   Definition rule := action nil unit_t.
 End Syntax.
 
